\documentclass[latex/main.tex]{subfiles}

\begin{document}
\section{Appendix}

\subsubsection{tmp}

notation:
\begin{align*}
    m(k, \tau) &= \text{exp}(-\frac{k}{\tau})\\
    m_{\tau,k}(k, \tau) &= \frac{\partial}{\partial \tau} m(k, \tau) = \frac{k}{\tau^2} \text{ exp}(-\frac{k}{\tau})\\
     m_{\tau\tau,k}(k, \tauz) &= \frac{\partial^2}{\partial \tau \partial \tau'} m(k, \tau) = \frac{x^2}{\tau^4} \text{ exp}(-\frac{k}{\tau}) - \frac{2k}{\tau^3} \text{ exp}(-\frac{k}{\tau})
\end{align*}

definition:
\begin{align*}
    S(\tau) &= \mathbb{E}[S_n(\tau)] = \mathbb{E}[(\rho - m(k, \tau))^2]\\
    \tau_0 &= \underset{\tau}{\text{argmin }} S(\tau)
\end{align*}

estimation:
\begin{align*}
    \hat{S}_n(\tau) &= \frac{1}{K} \sum_{k=1}^K (\rho_k - m(k, \tau))^2\\
    \hat \tau_{\text{nls}} &= \underset{\tau}{\text{argmin }} S_n(\tau)\\
    \hat e_k &= \rho_k - m(k, \hat \tau_{\text{nls}})
\end{align*}

consistency: 
\begin{align*}
    S_n(\tau) &\underset{p}{\to} S(\tau)\\
    \hat \tau_{\text{nls}} &\underset{p}{\to} \tau_0
\end{align*}

asymptotic distribution:
\begin{align*}
    Q &= \mathbb{E}[m_{\tau,k} m_{\tau, k}^{'}]\\
    \Omega &= \mathbb{E}[m_{\tau,k} m_{\tau, k}^{'} e_k^2]\\
    (\text{or } \Omega &= \sum_{\ell=-\infty}^{\infty} \mathbb{E}[??])\\
    \sqrt{K}(\hat\tau - \tau_0) &\underset{d}{\to} \mathcal{N}(0, Q^{-1} \Omega Q^{-1})
\end{align*}

variance estimation:
\begin{align*}
    \hat Q &= \frac{1}{K} \sum_{k=1}^K \frac{\partial^2}{\partial \tau \partial \tau'} m(k, \tau)\\
    \hat \Omega &= \frac{1}{K} \sum_{k=1}^{K} \hat m_{\tau,k}(k, \tau) \hat m_{\tau,k}^{'}(k, \tau) \hat e_k^2
\end{align*}
...

\end{document}